Foundation/Modal/Axioms.lean
@@ -34,7 +34,7 @@ protected abbrev P : F := ∼(□⊥)
 /-- Axiom for transivity -/
 protected abbrev Four := □φ ➝ □□φ
 
-protected abbrev FourN (n : ℕ+) (φ : F) := □^[n]φ ➝ □^[(n + 1)]φ
+protected abbrev FourN (n : ℕ) (φ : F) := □^[n]φ ➝ □^[(n + 1)]φ
 
 /-- Axiom for euclidean -/
 protected abbrev Five := ◇φ ➝ □◇φ
